No_sign_resp api abstraction steps function added

share/pulse/examples/dice/dpe/SPDM7.fst
@@ -249,6 +249,292 @@ fn extend_trace (gr: gref) (tr0: trace) (gs:g_state{valid_transition tr0 gs})
      
   }
 
+let state_change_success_no_sign (tr0:trace)
+                                 (tr1:trace)
+                     : prop =
+   (G_Recv_no_sign_resp? (current_state tr1)) /\
+   (valid_transition tr0 (current_state tr1)) /\ (tr1 == next_trace tr0 (current_state tr1)) /\
+   (G_Recv_no_sign_resp? (current_state tr1))
+
+let hash_result_success_no_sign (tr0:trace{has_full_state_info (current_state tr0)}) 
+                                (tr1:trace{has_full_state_info (current_state tr1) /\
+                                        has_full_state_info (previous_current_state tr1)})
+                                (#b_resp: Seq.seq u8{Seq.length b_resp > 0 /\ (UInt.fits (Seq.length b_resp) U32.n)})
+                                (#b_req: Seq.seq u8{Seq.length b_req > 0 /\ (UInt.fits (Seq.length b_req) U32.n)}) 
+                     : prop =
+  (exists hash_algo. 
+                  hash_of hash_algo (current_transcript tr0 ) 
+                  (U32.uint_to_t(Seq.length b_req)) 
+                  b_req 
+                  (U32.uint_to_t (Seq.length b_resp)) 
+                  b_resp 
+                  (current_transcript tr1))
+
+
+fn
+no_sign_resp_aux
+  (ctx:parser_context)
+  (req_size: u32{u32_v req_size > 0})
+  (req:V.vec u8 { V.length req == u32_v req_size })
+  (c:state)
+  (st:st)
+  (rep:repr)
+  (res:spdm_measurement_result_t)
+  (#tr0:trace {has_full_state_info (current_state tr0) })
+  (#b_resp: Seq.seq u8{Seq.length b_resp > 0 /\ Seq.length b_resp == u32_v ctx.resp_size /\
+                       (UInt.fits (Seq.length b_resp) U32.n)})
+  (#b_req: Seq.seq u8{Seq.length b_req > 0 /\ Seq.length b_req == u32_v req_size /\
+                      (UInt.fits (Seq.length b_req) U32.n)}) 
+  (#p_req : perm)
+  (#p_resp:perm)
+  requires parser_post1 ctx res false **
+           V.pts_to req #p_req b_req **
+           V.pts_to ctx.resp #p_resp b_resp **
+           V.pts_to st.session_transcript rep.transcript **
+           V.pts_to st.signing_pub_key rep.signing_pub_key_repr **
+           pure (st.key_size == rep.key_size_repr /\
+                (c == Initialized st \/ c == Recv_no_sign_resp st) /\
+                (rep.transcript == (current_transcript tr0)) /\
+                (rep.signing_pub_key_repr == (current_key tr0)) /\
+                (rep.key_size_repr == (current_key_size tr0)) /\
+                (G_Recv_no_sign_resp? (current_state tr0) \/ G_Initialized? (current_state tr0)) /\
+                res.status == Success) **
+           C.ghost_pcm_pts_to 
+                  (get_state_data c).g_trace_ref
+                  (Some #perm 1.0R, tr0)
+
+           
+  returns ret: spdm_measurement_result_t & state
+   
+   ensures  V.pts_to req #p_req b_req **
+            V.pts_to ctx.resp #p_resp b_resp **
+            parser_post1 ctx (fst ret) false **
+             (exists* tr1.
+                  spdm_inv (snd ret) (get_state_data (snd ret)).g_trace_ref tr1 **
+                  pure ((fst ret).status == Success ==>
+                                      state_change_success_no_sign tr0 tr1 /\
+                                      hash_result_success_no_sign tr0 tr1 #b_resp #b_req ))
+{
+   let curr_state_data = get_state_data c;
+    let curr_state_transcript:V.vec u8 = curr_state_data.session_transcript;
+    let curr_state_signing_pub_key = curr_state_data.signing_pub_key;
+    let curr_state_key_size = curr_state_data.key_size;
+      //get the ghost transcript
+    let curr_g_transcript = current_transcript tr0;
+      
+    let curr_g_key = current_key tr0;
+    let curr_g_key_size = current_key_size tr0;
+    
+    rewrite (V.pts_to st.session_transcript rep.transcript) as
+                  (V.pts_to curr_state_transcript rep.transcript);
+        
+    rewrite (V.pts_to curr_state_transcript rep.transcript) as
+                (V.pts_to curr_state_transcript curr_g_transcript);
+    
+    assert_ (pure(Seq.length curr_g_transcript == hash_size));
+    let new_g_transcript' = hash_seq hash_algo curr_g_transcript req_size b_req;
+    let new_g_transcript = hash_seq hash_algo new_g_transcript' ctx.resp_size b_resp;
+    
+    assert_ (pure(V.length curr_state_transcript == hash_size));
+    assert_ (V.pts_to curr_state_transcript curr_g_transcript);
+    assert_ (V.pts_to req #p_req b_req);
+    
+     hash hash_algo curr_state_transcript req_size req #curr_g_transcript #b_req #p_req;
+     assert_ (pure (Seq.equal new_g_transcript' (hash_seq hash_algo curr_g_transcript req_size b_req)));
+     assert_ (V.pts_to curr_state_transcript new_g_transcript');
+     hash hash_algo curr_state_transcript ctx.resp_size ctx.resp #new_g_transcript' #b_resp #p_resp;
+     assert_ (V.pts_to curr_state_transcript new_g_transcript);
+     
+     //create a new state data record with the new transcript
+    //creation of the ghost session data storage
+    let rep_new = {key_size_repr = curr_g_key_size; signing_pub_key_repr = curr_g_key; transcript = new_g_transcript};
+         
+    //Trace ref creation-----------------------------------------------------------------------------------------------------------
+    //new trace----------------------------------------------------------------------------------------------------------------
+    //bring in a lemma to prove this
+    assume_ (pure(valid_transition tr0 (G_Recv_no_sign_resp rep_new)));
+
+    let tr1 = next_trace tr0 (G_Recv_no_sign_resp rep_new);
+
+    assert (pure(exists hash_algo. 
+                        hash_of hash_algo (current_transcript tr0 ) 
+                        (U32.uint_to_t(Seq.length b_req)) 
+                        b_req 
+                        (U32.uint_to_t (Seq.length b_resp)) 
+                        b_resp 
+                        (current_transcript tr1)));
+
+
+  
+    assert_ (pure (valid_transition tr0 (G_Recv_no_sign_resp rep_new)));
+    extend_trace ((get_state_data c).g_trace_ref) tr0 ((G_Recv_no_sign_resp rep_new));
+        
+    //New state data record creation
+    //----------------------------------------------------------------------------------------------------------------------------
+    let new_st = {key_size = curr_state_key_size; 
+                    signing_pub_key = curr_state_signing_pub_key; 
+                    session_transcript = curr_state_transcript;
+                    g_trace_ref = curr_state_data.g_trace_ref};
+
+    //Do the state change---------------------------------------------------------------------------------------------------------
+    let new_state = (Recv_no_sign_resp new_st);
+
+    assert_ (pure (res.status == Success ==> (G_Recv_no_sign_resp? (current_state tr1) /\
+                            valid_transition tr0 (current_state tr1) /\ tr1 == next_trace tr0 (current_state tr1)) /\
+                           (G_Recv_no_sign_resp? (current_state tr1) /\
+                           (exists hash_algo. 
+                                   hash_of hash_algo (current_transcript tr0 ) 
+                                  (U32.uint_to_t(Seq.length b_req)) 
+                                  b_req 
+                                  (U32.uint_to_t (Seq.length b_resp)) 
+                                  b_resp 
+                                 (current_transcript tr1)))));
+
+  
+     with _v. rewrite (V.pts_to curr_state_transcript _v) as
+                         (V.pts_to curr_state_transcript new_g_transcript);
+        
+     rewrite (V.pts_to curr_state_transcript new_g_transcript) as
+                (V.pts_to new_st.session_transcript rep_new.transcript);
+
+     rewrite (V.pts_to st.signing_pub_key rep.signing_pub_key_repr) as
+                (V.pts_to curr_state_signing_pub_key rep.signing_pub_key_repr);
+        
+     rewrite (V.pts_to curr_state_signing_pub_key rep.signing_pub_key_repr) as
+                (V.pts_to curr_state_signing_pub_key curr_g_key);
+
+     rewrite (V.pts_to curr_state_signing_pub_key curr_g_key) as
+                (V.pts_to new_st.signing_pub_key rep_new.signing_pub_key_repr);
+
+     assert_ ( V.pts_to new_st.signing_pub_key rep_new.signing_pub_key_repr **
+                  V.pts_to new_st.session_transcript rep_new.transcript **
+                  pure (new_st.key_size == rep_new.key_size_repr));
+
+     fold (session_state_related (Recv_no_sign_resp new_st) (G_Recv_no_sign_resp rep_new));
+
+     with _v. rewrite (C.ghost_pcm_pts_to #trace_pcm_t #trace_pcm _v (pcm_elt 1.0R tr1)) as
+                         (C.ghost_pcm_pts_to (get_state_data (Recv_no_sign_resp new_st)).g_trace_ref (pcm_elt 1.0R tr1));
+
+     fold (spdm_inv (Recv_no_sign_resp new_st) (get_state_data (Recv_no_sign_resp new_st)).g_trace_ref tr1);
+        
+     let fin = (res, new_state);
+        
+     fin
+}
+
+
+fn no_sign_resp1
+  (ctx:parser_context)
+  (req_size: u32{u32_v req_size > 0})
+  (req:V.vec u8 { V.length req == u32_v req_size })
+  (c:state)
+  (#tr0:trace{has_full_state_info (current_state tr0)})
+  (#b_resp: G.erased (Seq.seq u8){u32_v ctx.resp_size > 0 /\ Seq.length b_resp == u32_v ctx.resp_size})
+  (#b_req: G.erased (Seq.seq u8){Seq.length b_req == u32_v req_size})
+  (#p_req : perm)
+  (#p_resp:perm)
+   requires (V.pts_to req #p_req b_req **
+             V.pts_to ctx.resp #p_resp b_resp) **
+             spdm_inv c ((get_state_data c).g_trace_ref) tr0 **
+             pure (G_Recv_no_sign_resp? (current_state tr0) \/ G_Initialized? (current_state tr0))
+    returns res: spdm_measurement_result_t & state
+    
+    ensures V.pts_to req #p_req b_req **
+            V.pts_to ctx.resp #p_resp b_resp **
+
+            //parser related post-conditions
+            parser_post1 ctx (fst res) false  **
+           
+            //state change related post-condition 
+             (exists* tr1.
+                     spdm_inv (snd res) (get_state_data (snd res)).g_trace_ref tr1 **
+                     (*no_sign_resp_state_related_post_conditions ctx tr0 tr1 c (snd res) #b_resp #b_req (fst res)*)
+                     pure ((fst res).status == Success ==> (G_Recv_no_sign_resp? (current_state tr1)) /\
+                            (valid_transition tr0 (current_state tr1)) /\ (tr1 == next_trace tr0 (current_state tr1)) /\
+                           (G_Recv_no_sign_resp? (current_state tr1)) /\
+
+                           (exists hash_algo. 
+                                   hash_of hash_algo (current_transcript tr0 ) 
+                                  (U32.uint_to_t(Seq.length b_req)) 
+                                  b_req 
+                                  (U32.uint_to_t (Seq.length b_resp)) 
+                                  b_resp 
+                                 (current_transcript tr1))))
+
+            
+{
+  let res = parser0 ctx #p_resp #b_resp false;
+  match res.status {
+    Parse_error -> {
+      let tr1 = tr0;
+      let r = (get_state_data c).g_trace_ref;
+      assert (spdm_inv c ((get_state_data c).g_trace_ref) tr0);
+      assert (spdm_inv c (get_state_data c).g_trace_ref tr1);
+
+      rewrite 
+        (spdm_inv c ((get_state_data c).g_trace_ref) tr0) as
+        (spdm_inv c (get_state_data c).g_trace_ref tr1);
+      
+      assert_ (pure (res.status == Success ==> (G_Recv_no_sign_resp? (current_state tr1) /\
+               valid_transition tr0 (current_state tr1) /\ tr1 == next_trace tr0 (current_state tr1)) /\
+              (G_Recv_no_sign_resp? (current_state tr1) /\
+              (exists hash_algo. 
+                                   hash_of hash_algo (current_transcript tr0 ) 
+                                  (U32.uint_to_t(Seq.length b_req)) 
+                                  b_req 
+                                  (U32.uint_to_t (Seq.length b_resp)) 
+                                  b_resp 
+                                 (current_transcript tr1))
+              )));
+       (res,c)
+    }
+    Success -> {
+       //current state transcript
+      let curr_state_data = get_state_data c;
+      let curr_state_transcript:V.vec u8 = curr_state_data.session_transcript;
+      let curr_state_signing_pub_key = curr_state_data.signing_pub_key;
+      let curr_state_key_size = curr_state_data.key_size;
+      //get the ghost transcript
+      let curr_g_transcript = current_transcript tr0;
+      
+      let curr_g_key = current_key tr0;
+      let curr_g_key_size = current_key_size tr0;
+      
+      //assert (spdm_inv c ((get_state_data c).g_trace_ref) tr0);
+      unfold (spdm_inv c ((get_state_data c).g_trace_ref) tr0);
+      
+      //assert (session_state_related c (current_state tr0));
+      unfold (session_state_related c (current_state tr0));
+      
+      let rep = get_gstate_data (current_state tr0);
+      match c {
+        Initialized st -> {
+          intro_session_state_tag_related (Initialized st) (current_state tr0);
+          rewrite (session_state_related (Initialized st) (current_state tr0)) as
+                 (session_state_related (Initialized st) (G_Initialized rep));
+
+        
+          unfold (session_state_related (Initialized st) (G_Initialized rep));
+        
+        
+          admit()
+        }
+         Recv_no_sign_resp st ->{
+          intro_session_state_tag_related (Recv_no_sign_resp st ) (current_state tr0);
+          rewrite (session_state_related (Recv_no_sign_resp st) (current_state tr0)) as
+                 (session_state_related (Recv_no_sign_resp st) (G_Recv_no_sign_resp rep));
+          
+          unfold (session_state_related (Recv_no_sign_resp st) (G_Recv_no_sign_resp rep));
+        
+          admit()
+          
+         }
+      }
+    }
+  }
+}
+
+
 fn no_sign_resp1
   (ctx:parser_context)
   (req_size: u32{u32_v req_size > 0})
@@ -344,7 +630,7 @@ fn no_sign_resp1
         
         
           rewrite (V.pts_to st.session_transcript rep.transcript) as
-                (V.pts_to curr_state_transcript rep.transcript);
+                  (V.pts_to curr_state_transcript rep.transcript);
         
         
 
